Work in progress to cut some dependency on extlib, use a shallower eitherT monad transformer, clean up/ think a bit more about the monad infrastructure we are building and draft an Interpretable type class

theories/Basics/Monad.v
@@ -4,9 +4,6 @@
 From Coq Require Import
      Morphisms.
 
-From ExtLib Require Export
-     Structures.Monad.
-
 From ITree Require Import
      Basics.Basics
      Basics.CategoryOps
@@ -14,6 +11,24 @@ From ITree Require Import
 (* end hide *)
 
 Set Primitive Projections.
+(* Set Implicit Arguments. *)
+(* Set Strict Implicit. *)
+(* Set Universe Polymorphism. *)
+
+Set Implicit Arguments.
+Set Strict Implicit.
+
+Polymorphic Class Functor@{d c} (F : Type@{d} -> Type@{c}) : Type :=
+  { fmap : forall {A B : Type@{d}}, (A -> B) -> F A -> F B }.
+
+Module FunctorNotation.
+  Notation "f <$> x" := (@fmap _ _ _ _ f x) (at level 52, left associativity).
+End FunctorNotation.
+
+Class Monad@{d c} (m : Type@{d} -> Type@{c}) : Type :=
+{ ret : forall {t : Type@{d}}, t -> m t
+; bind : forall {t u : Type@{d}}, m t -> (t -> m u) -> m u
+}.
 
 Class EqM (m:Type -> Type) : Type :=
   eqm : forall a, m a -> m a -> Prop.
@@ -24,7 +39,65 @@ Class EqMProps (m:Type -> Type) `{Monad m} `{EqM m} :=
 Arguments eqm {m _ _}.
 Infix "≈" := eqm (at level 70) : monad_scope.
 
-Section Laws.
+Section monadic.
+
+  Definition liftM@{d c}
+              {m : Type@{d} -> Type@{c}}
+              {M : Monad m}
+              {T U : Type@{d}} (f : T -> U) : m T -> m U :=
+    fun x => bind x (fun x => ret (f x)).
+
+  Definition liftM2@{d c}
+              {m : Type@{d} -> Type@{c}}
+              {M : Monad m}
+              {T U V : Type@{d}} (f : T -> U -> V) : m T -> m U -> m V :=
+    Eval cbv beta iota zeta delta [ liftM ] in
+      fun x y => bind x (fun x => liftM (f x) y).
+
+  Definition liftM3@{d c}
+              {m : Type@{d} -> Type@{c}}
+              {M : Monad m}
+              {T U V W : Type@{d}} (f : T -> U -> V -> W) : m T -> m U -> m V -> m W :=
+    Eval cbv beta iota zeta delta [ liftM2 ] in
+      fun x y z => bind x (fun x => liftM2 (f x) y z).
+
+  Definition apM@{d c}
+              {m : Type@{d} -> Type@{c}}
+              {M : Monad m}
+              {A B : Type@{d}} (fM:m (A -> B)) (aM:m A) : m B :=
+    bind fM (fun f => liftM f aM).
+
+  (* Left-to-right composition of Kleisli arrows. *)
+  Definition mcompose@{c d}
+             {m:Type@{d}->Type@{c}}
+             {M: Monad m}
+             {T U V:Type@{d}}
+             (f: T -> m U) (g: U -> m V): (T -> m V) :=
+    fun x => bind (f x) g.
+
+End monadic.
+
+Module MonadNotation.
+
+  Delimit Scope monad_scope with monad.
+
+  Notation "c >>= f" := (@bind _ _ _ _ c f) (at level 58, left associativity) : monad_scope.
+  Notation "f =<< c" := (@bind _ _ _ _ c f) (at level 61, right associativity) : monad_scope.
+  Notation "f >=> g" := (@mcompose _ _ _ _ _ f g) (at level 61, right associativity) : monad_scope.
+
+  Notation "x <- c1 ;; c2" := (@bind _ _ _ _ c1 (fun x => c2))
+    (at level 61, c1 at next level, right associativity) : monad_scope.
+
+  Notation "e1 ;; e2" := (_ <- e1%monad ;; e2%monad)%monad
+    (at level 61, right associativity) : monad_scope.
+
+  Notation "' pat <- c1 ;; c2" :=
+    (@bind _ _ _ _ c1 (fun x => match x with pat => c2 end))
+    (at level 61, pat pattern, c1 at next level, right associativity) : monad_scope.
+
+End MonadNotation.
+
+Section MonadLaws.
 
   Context (m : Type -> Type).
   Context {EqM : @EqM m}.
@@ -32,21 +105,119 @@ Section Laws.
   Context {EqMP : @EqMProps m _ EqM}.
 
   Local Open Scope monad_scope.
-  
-  (* This should go coq-ext-lib. *)
+
   Class MonadLaws :=
-    { bind_ret_l :> forall a b (f : a -> m b) (x : a), bind (ret x) f ≈ f x
-    ; bind_ret_r :> forall a (x : m a), bind x (fun y => ret y) ≈ x
-    ; bind_bind :> forall a b c (x : m a) (f : a -> m b) (g : b -> m c), bind (bind x f) g ≈ bind x (fun y => bind (f y) g)
+    { bind_ret_l : forall a b (f : a -> m b) (x : a), bind (ret x) f ≈ f x
+    ; bind_ret_r : forall a (x : m a), bind x (fun y => ret y) ≈ x
+    ; bind_bind : forall a b c (x : m a) (f : a -> m b) (g : b -> m c), bind (bind x f) g ≈ bind x (fun y => bind (f y) g)
     ; Proper_bind :> forall {a b},
         (@Proper (m a%type -> (a -> m b) -> m b)
          (eqm ==> pointwise_relation _ eqm ==> eqm)
          bind)
     }.
 
-End Laws.
+End MonadLaws.
 
 Arguments bind_ret_l {m _ _ _}.
 Arguments bind_ret_r {m _ _ _}.
 Arguments bind_bind {m _ _ _}.
 Arguments Proper_bind {m _ _ _}.
+
+(** ** Loop operator *)
+
+(** [iter]: A primitive for general recursion.
+    Iterate a function updating an accumulator [I], until it produces
+    an output [R].
+ *)
+Polymorphic Class MonadIter (M : Type -> Type) : Type :=
+  iter : forall {R I: Type}, (I -> M (I + R)%type) -> I -> M R.
+
+(* Its laws are defined by its [Kleisli] category forming an [Iterative] category *)
+
+Section MonadHomomorphism.
+
+  Local Open Scope monad_scope.
+
+  Variable M M': Type -> Type.
+  Context {MM: Monad M}.
+  Context {MM': Monad M'}.
+  Context {IM: MonadIter M}.
+  Context {IM': MonadIter M'}.
+  Context {EqMM': @EqM M'}.
+  Variable F: M ~> M'.
+
+  Class MonadHom: Prop :=
+    {
+      resp_ret : forall A (a: A), F (ret a) ≈ ret a;
+      resp_bind: forall A B (m: M A) (k: A -> M B),
+          F (bind m k) ≈ bind (F m) (fun x => F (k x))
+    }.
+
+  Class IterHom: Prop :=
+    {
+      resp_iter: forall (I R: Type) (body: I -> M (I + R)%type) i,
+        F (iter body i) ≈ iter (fun x => F (body x)) i
+    }.
+
+End MonadHomomorphism.
+
+Section MonadTriggerable.
+
+  Local Open Scope monad_scope.
+
+  Variable M M': Type -> Type.
+  Context {MM: Monad M}.
+  Context {MM': Monad M'}.
+  Context {EqMM': @EqM M'}.
+  Context {IM: MonadIter M}. 
+  Context {IM': MonadIter M'}.
+
+  (**
+     Monads that allow for the embedding of an effect as a minimal
+     monadic effectful computation are dubbed "Triggerable".
+   *)
+
+  Class Triggerable := trigger: forall (E: Type -> Type), E ~> M.
+
+  (* The correctness of this operation, i.e. its minimality, is expressed
+     with respect to a notion of interpretation of monads.
+     A monad [M] is said to be "Interpretable" into a monad [M'] if there
+     is a family of monad monomorphisms for each handler [h: E ~> M'].
+   *)
+
+  Class Interpretable :=
+    interp: forall (E: Type -> Type) (h: E ~> M'), M ~> M'.
+
+  Class InterpCorrect {InterpMM': Interpretable} {TrigM: Triggerable}: Prop :=
+    {
+      interp_monad_hom E h :> MonadHom (interp E h);
+      interp_iter_hom  E h :> IterHom (interp E h);
+      interp_trigger E h T (e: E T): interp E h (trigger _ _ e) ≈ h _ e
+    }.
+
+End MonadTriggerable.
+
+Import CatNotations.
+Local Open Scope cat_scope.
+Local Open Scope monad_scope.
+
+Ltac rw_pointed_l H :=
+  match goal with
+    |- ?f ?x ≈ _ =>
+    let tmp := fresh "H" in
+    assert (tmp: f ⩯ f) by reflexivity;
+    setoid_rewrite H in tmp at 1;
+    specialize (tmp x);
+    setoid_rewrite <- tmp
+  end.
+
+Ltac rw_pointed_r H :=
+  match goal with
+    |- _ ≈ ?f ?x =>
+    let tmp := fresh "H" in
+    assert (tmp: f ⩯ f) by reflexivity;
+    setoid_rewrite H in tmp at 1;
+    specialize (tmp x);
+    setoid_rewrite <- tmp
+  end.
+
