theories/Basics/MonadEither.v
@@ -2,10 +2,6 @@ From Coq Require Import
      Setoid
      Morphisms.
 
-From ExtLib Require Import
-     Structures.Monad
-     EitherMonad.
-
 From ITree Require Import
      Basics.Basics
      Basics.Category
@@ -13,144 +9,171 @@ From ITree Require Import
      Basics.CategoryKleisliFacts
      Basics.Monad.
 
-Import ITree.Basics.Basics.Monads.
 Import CatNotations.
+Import MonadNotation.
 Local Open Scope cat_scope.
 Local Open Scope cat.
+Local Open Scope monad_scope.
 
-Section Either.
+Definition eitherT (exn: Type) (M: Type -> Type) (a: Type) : Type :=
+  M (sum exn a).
+Definition either (exn a : Type) : Type :=
+  sum exn a.
+
+Section Functor_Either.
+  Global Instance Functor_eitherT {M} {Fm : Functor M} (exn: Type) : Functor (eitherT exn M)
+    := {|
+        fmap _ _ f :=  fmap (fun ma => match ma with
+                                    | inl e => inl e
+                                    | inr a => inr (f a)
+                                    end)
+      |}.
+
+End Functor_Either.
+
+Section Monad_Either.
   Variable M : Type -> Type.
-  Variable A : Type.
+  Variable exn : Type.
   Context {EQM : EqM M}.
   Context {HM: Monad M}.
   Context {HEQP: @EqMProps M _ EQM}.
   Context {ML: @MonadLaws M _ HM}.
 
-  Global Instance EqM_eitherTM : EqM (eitherT A M).
-  Proof.
-    intros ? [a] [b].
-    exact (eqm a b).
-  Defined.
+  Global Instance Monad_eitherT : Monad (eitherT exn M)
+    := {|
+        ret _ a := ret (inr a)
+        ; bind _ _ t k :=
+            bind (m := M) t
+                 (fun ma =>
+                    match ma with
+                    | inl e => ret (inl e)
+                    | inr a => k a
+                    end)
+      |}.
 
-  Global Instance EqMProps_eitherTM : @EqMProps (eitherT A M) _ EqM_eitherTM.
+  Global Instance EqM_eitherTM : EqM (eitherT exn M) := fun _ => eqm (m := M).
+
+  Global Instance EqMProps_eitherTM : @EqMProps _ _ EqM_eitherTM.
   Proof.
   constructor.
-  - intros [x]; cbn; reflexivity.
-  - intros [x] [y]; cbn; symmetry; auto.
-  - intros [x] [y] [z]; cbn; etransitivity; eauto.
+  - repeat red; reflexivity.
+  - repeat red; intros x y; cbn; symmetry; auto.
+  - repeat red; intros x y z; cbn; etransitivity; eauto.
   Qed.
 
-  Instance MonadLaws_eitherTM : @MonadLaws (eitherT A M) _ _.
+  Instance MonadLaws_eitherTM : @MonadLaws (eitherT exn M) _ _.
   Proof.
   constructor.
-  - cbn. intros a b f x; destruct (f x) eqn:EQ.
+  - cbn. intros a b f x.
     repeat red.
-    rewrite bind_ret_l, EQ; cbn.
+    rewrite bind_ret_l; cbn.
     reflexivity.
-  - cbn. intros a [x]; cbn.
+  - cbn; intros a x. unfold eitherT in x.
+    unfold eqm, EqM_eitherTM.
     match goal with
       |- _ ≈ ?h => rewrite <- (bind_ret_r _ h) at 2
     end.
     apply Proper_bind; [reflexivity | intros [b | m]; reflexivity].
-  - cbn. intros a b c [x] f g; cbn.
-    rewrite bind_bind.
+  - cbn. intros a b c x f g; cbn.
+    rewrite bind_bind. do 2 red.
     apply Proper_bind; [reflexivity | intros [? | m]].
     + rewrite bind_ret_l; reflexivity.
     + reflexivity.
-  - cbn; intros a b [x] [y] EQ x' y' H'; cbn in *.
-    apply Proper_bind; [auto | intros [? | ?]]; [reflexivity |].
-    specialize (H' a0).
-    destruct (x' a0), (y' a0); cbn in *; auto.
+  - cbn; intros a b x y EQ x' y' H'; cbn in *.
+    do 2 red; apply Proper_bind; [auto | intros [? | ?]]; [reflexivity | apply H'].
   Qed.
 
-  Context {IM: Iter (Kleisli M) sum}.
+End Monad_Either.
+
+Section Iter_Either.
+
+  Variable M : Type -> Type.
+  Variable exn : Type.
+  Context {EQM : EqM M}.
+  Context {HM: Monad M}.
+  Context {HEQP: @EqMProps M _ EQM}.
+  Context {ML: @MonadLaws M _ HM}.
+  Context {IM: MonadIter M}.
   Context {CM: Iterative (Kleisli M) sum}.
 
-  Definition iso {a b:Type} (Aab : A + (a + b)) : (a  + (A + b)) :=
+  Definition iso {a b:Type} (Aab : exn + (a + b)) : (a  + (exn + b)) :=
     match Aab with
     | inl A => inr (inl A)
     | inr (inl a) => inl a
     | inr (inr b) => inr (inr b)
     end.
 
-  Definition internalize {a b:Type} (f : Kleisli (eitherT A M) a b) : Kleisli M a (A + b) :=
-    fun x => let '(mkEitherT y) := f x in y.
+  Definition internalize {a b:Type} (f : Kleisli (eitherT exn M) a b) : Kleisli M a (exn + b) := f.
 
-  Global Instance Iter_eitherTM : Iter (Kleisli (eitherT A M)) sum :=
-    fun (a b: Type) (f: a -> (eitherT A M (a + b))) x =>
-      mkEitherT (iter ((internalize f) >>> (pure iso)) x).
+  Global Instance Iter_eitherTM : MonadIter (eitherT exn M) :=
+    fun (b a: Type) (f: a -> M (exn + (a + b))) x =>
+      iter ((internalize f) >>> (pure iso)) x.
 
   Instance proper_internalize {a b}: Proper (eq2 ==> eq2) (@internalize a b).
-  intros x y H o; specialize (H o).
-  unfold internalize; destruct (x o), (y o).
-  apply H.
+  intros x y H o; apply H.
   Qed.
 
-  Global Instance Proper_Iter_eitherTM : forall a b, @Proper (Kleisli (eitherT A M) a (a + b) -> (Kleisli (eitherT A M) a b)) (eq2 ==> eq2) iter.
+  Global Instance Proper_Iter_eitherTM : forall a b, @Proper (Kleisli (eitherT exn M) a (a + b) -> (Kleisli (eitherT exn M) a b)) (eq2 ==> eq2) iter.
   Proof.
     destruct CM.
-    intros a b x y H a0.
+    intros A B x y H a.
     apply iterative_proper_iter.
     apply cat_eq2_r.
     rewrite H; reflexivity.
- Qed.
+  Qed.
 
-  Global Instance IterUnfold_eitherTM : IterUnfold (Kleisli (eitherT A M)) sum.
+  Global Instance IterUnfold_eitherTM : IterUnfold (Kleisli (eitherT exn M)) sum.
   Proof.
-    destruct CM.
-    intros a b f o.
-    cbn; destruct (f o) as [e] eqn:EQ; cbn.
+    intros A B f a; cbn.
+    unfold CategoryOps.iter, Iter_Kleisli.
+    rewrite iter_monad_to_cat.
+    rw_pointed_l iter_unfold.
     unfold cat, Cat_Kleisli.
-    unfold iter, Iter_eitherTM.
-    rewrite iterative_unfold.
-    unfold cat, Cat_Kleisli.
+    do 2 red.
     rewrite bind_bind.
     apply Proper_bind.
-    + unfold internalize; rewrite EQ; reflexivity.
+    + reflexivity.
     + intros [xA | [xa | xb]]; unfold pure; rewrite bind_ret_l; reflexivity.
   Qed.
 
-  Global Instance IterNatural_eitherTM : IterNatural (Kleisli (eitherT A M)) sum.
+  Global Instance IterNatural_eitherTM : IterNatural (Kleisli (eitherT exn M)) sum.
   Proof.
     destruct CM.
-    intros a b c f g o.
-    cbn; destruct (f o) as [e] eqn:EQf; cbn.
+    intros A B C f g a; cbn.
     setoid_rewrite iterative_natural.
     apply iterative_proper_iter; intros a'.
     unfold cat, Cat_Kleisli.
-    unfold internalize; destruct (f a') eqn:EQf'; cbn.
+    unfold internalize; cbn.
     rewrite! bind_bind.
     apply Proper_bind; [reflexivity |].
     intros [xA | [xa | xb]]; unfold pure; cbn; rewrite !bind_ret_l; cbn; unfold cat, Cat_Kleisli; cbn.
     - rewrite bind_ret_l; cbn; reflexivity.
-    - unfold id_, Id_Kleisli, pure; rewrite bind_ret_l; reflexivity.
-    - destruct (g xb); cbn; rewrite bind_bind.
+    - unfold id_, Id_Kleisli, pure; rewrite bind_bind, !bind_ret_l; reflexivity.
+    - cbn; rewrite bind_bind.
       apply Proper_bind; [reflexivity |].
       intros [? | ?]; rewrite bind_ret_l; reflexivity.
   Qed.
 
   Lemma iter_dinatural_helper:
-    forall (a b c : Type) (f : Kleisli (eitherT A M) a (b + c)) (g : Kleisli (eitherT A M) b (a + c)),
+    forall (a b c : Type) (f : Kleisli (eitherT exn M) a (b + c)) (g : Kleisli (eitherT exn M) b (a + c)),
       internalize (f >>> case_ g inr_) >>> pure iso ⩯ internalize f >>> pure iso >>> case_ (internalize g >>> pure iso) inr_.
   Proof.
     destruct CM.
     intros a b c f g o.
     unfold cat, Cat_Kleisli, internalize; cbn.
-    repeat rewrite bind_bind.
-    destruct (f o) as [fo] eqn: EQ; cbn.
+    repeat rewrite bind_bind; cbn.
     unfold pure; cbn.
     apply Proper_bind; [reflexivity | intros [xA | [xa | xb]]]; cbn.
     - rewrite !bind_ret_l; reflexivity.
-    - destruct (g xa) as [gxa] eqn:EQ'; cbn.
-      rewrite bind_ret_l; cbn; rewrite EQ'; reflexivity.
+    - rewrite bind_ret_l; reflexivity.
     - rewrite !bind_ret_l; reflexivity.
   Qed.
 
-  Global Instance IterDinatural_eitherTM : IterDinatural (Kleisli (eitherT A M)) sum.
+  Global Instance IterDinatural_eitherTM : IterDinatural (Kleisli (eitherT exn M)) sum.
   Proof.
     destruct CM.
     unfold IterDinatural.
-    intros a b c f g o.
+    intros A B C f g a.
     unfold iter, Iter_eitherTM. cbn.
     eapply transitivity.
     eapply iterative_proper_iter.
@@ -160,6 +183,7 @@ Section Either.
     unfold cat, Cat_Kleisli.
     rewrite bind_bind.
     unfold internalize. cbn.
+    do 2 red.
     apply Proper_bind.
     - reflexivity.
     - unfold pure; cbn; intros [xA | [xa | xb]]; cbn.
@@ -167,13 +191,12 @@ Section Either.
       + rewrite bind_ret_l; cbn.
         eapply iterative_proper_iter.
         intros ?; rewrite !bind_bind.
-        destruct (g a0) eqn:EQ; cbn.
         apply Proper_bind; [reflexivity | intros [|[|]]]; cbn; rewrite !bind_ret_l; try reflexivity.
       + rewrite bind_ret_l; cbn.
         reflexivity.
   Qed.
 
-  Global Instance IterCodiagonal_eitherTM : IterCodiagonal (Kleisli (eitherT A M)) sum.
+  Global Instance IterCodiagonal_eitherTM : IterCodiagonal (Kleisli (eitherT exn M)) sum.
   Proof.
     destruct CM.
     unfold IterCodiagonal.
@@ -186,24 +209,36 @@ Section Either.
     unfold internalize; cbn. reflexivity.
     eapply transitivity.
 
-   eapply iterative_proper_iter.
-   apply iterative_natural.
-   rewrite iterative_codiagonal.
-   eapply iterative_proper_iter.
-   rewrite cat_assoc, bimap_case, cat_id_l, cat_id_r.
-   unfold internalize.
-   intros o'; cbn.
-   unfold cat, Cat_Kleisli; rewrite !bind_bind; destruct (f o'); cbn.
-   apply Proper_bind; [reflexivity | intros [| [|]]].
-   unfold pure; rewrite !bind_ret_l; reflexivity.
-   unfold pure; cbn; rewrite !bind_ret_l; reflexivity.
-   unfold pure; cbn; rewrite !bind_ret_l; reflexivity.
+    eapply iterative_proper_iter.
+    apply iterative_natural.
+    rewrite iterative_codiagonal.
+    eapply iterative_proper_iter.
+    rewrite cat_assoc, bimap_case, cat_id_l, cat_id_r.
+    unfold internalize.
+    intros o'; cbn.
+    unfold cat, Cat_Kleisli; cbn; rewrite !bind_bind; cbn.
+    apply Proper_bind; [reflexivity | intros [| [|]]].
+    unfold pure; rewrite !bind_ret_l; reflexivity.
+    unfold pure; cbn; rewrite !bind_ret_l; reflexivity.
+    unfold pure; cbn; rewrite !bind_ret_l; reflexivity.
   Qed.
 
-  Global Instance Iterative_eitherTM : Iterative (Kleisli (eitherT A M)) sum.
+  Global Instance Iterative_eitherTM : Iterative (Kleisli (eitherT exn M)) sum.
   Proof.
   constructor;
   typeclasses eauto.
   Qed.
 
-End Either.
+End Iter_Either.
+
+(* Section Interpretable_Either. *)
+
+(*   Variable M : Type -> Type. *)
+(*   Variable exn : Type. *)
+(*   Context {EQM : EqM M}. *)
+(*   Context {HM: Monad M}. *)
+(*   Context {HEQP: @EqMProps M _ EQM}. *)
+(*   Context {ML: @MonadLaws M _ HM}. *)
+(*   Context {IM: MonadIter M}. *)
+(*   Context {CM: Iterative (Kleisli M) sum}. *)
+
