theories/Events/State.v
@@ -9,6 +9,7 @@ From ExtLib Require Import
 
 From ITree Require Import
      Basics.Basics
+     Basics.MonadState
      Basics.CategoryOps
      Basics.CategoryKleisli
      Core.ITreeDefinition
